stlc internal

TaplLean/STLC/Env.lean
@@ -1,4 +1,11 @@
-import Batteries.Data.AssocList
-open Lean
+abbrev Env (α : Type) := String → Option α
 
-abbrev Env (α : Type) := AssocList String α
+def empty {α : Type} : (Env α) := fun _ => none
+
+def update {α : Type}
+  (x : String) (v : α) (env : Env α) : Env α
+  :=
+  fun y => if x = y then some v else env y
+
+notation:100 x " |→ " v " ; " τ => update x v τ
+notation:100 x " |→ " v => update x v empty
