TaplLean/STLC/Internal.lean
@@ -1,15 +1,46 @@
+import TaplLean.STLC.Env
+
 inductive Ty : Type where
   | TBool
   | TArrow : Ty → Ty → Ty
 
-infix:100 " T.-> " => Ty.TArrow
+infixr:50 " :-> " => Ty.TArrow
+
+abbrev TyEnv := Env Ty
 
 inductive Term : Type where
   | tru
   | fls
   | ite : Term → Term → Term → Term
   | var : String → Term
-  | abs : String → Ty → Term
+  | abs : String → Ty → Term → Term
   | app : Term → Term → Term
 
-inductive WellTyped : Term → Ty → Prop where
+notation:90 "λ" x " : " T " , " t => Term.abs x T t
+
+inductive WellTyped : TyEnv → Term → Ty → Prop where
+  | wt_tru : ∀ Γ, WellTyped Γ Term.tru TBool
+  | wt_fls : ∀ Γ, WellTyped Γ Term.fls TBool
+  | wt_ite : ∀ Γ t1 t2 t3 T,
+      WellTyped Γ t1 TBool →
+      WellTyped Γ t2 T →
+      WellTyped Γ t3 T →
+      WellTyped Γ (Term.ite t1 t2 t3) T
+  | wt_var : ∀ Γ x T, Γ x = some T → WellTyped Γ (Term.var x) T
+  | wt_abs : ∀ Γ x t1 T1 T2,
+      WellTyped (x |→ T2; Γ) t1 T1 →
+      WellTyped Γ (λ x : T2 , t1) (T2 :-> T1)
+  | wt_app : ∀ Γ t1 t2 T1 T2,
+      WellTyped Γ t1 (T2 :-> T1) →
+      WellTyped Γ t2 T2 →
+      WellTyped Γ (Term.app t1 t2) T1
+
+notation:100 Γ " ⊢ " t " ∈: " T => WellTyped Γ t T
+
+open WellTyped
+example : empty ⊢ (Term.app (λ x : TBool, Term.var x) Term.tru) ∈: TBool
+  := by
+  apply wt_app empty (λ x : TBool, Term.var x) Term.tru
+  . apply wt_abs empty x (Term.var x) TBool TBool
+    apply wt_var; simp [update]
+  . apply wt_tru
